examples/byte_register.thy
@@ -7,37 +7,49 @@ which doubles the value in the register, if possible.
 *)
 
 theory byte_register
-  imports Main "../Banks/banks" (*NO_CI*)
-  (*CI_ONLY imports Main "Banks.banks" CI_ONLY*)
+  imports "HOL-Library.Word" "../Banks/banks"  (*NO_CI*)
+  (*CI_ONLY imports "HOL-Library.Word" "Banks.banks"  CI_ONLY*)
 begin
 
+unbundle UTP_Syntax
+unbundle Expression_Syntax
+
+type_synonym bit = "1 word"
+
 alphabet \<alpha>ST = 
-  reg :: int
-  err :: int
+  reg :: "8 word"
+  err :: bit
 
 alphabet \<alpha>H =
-  reg\<^sub>H :: int
-  err\<^sub>H :: int
+  reg\<^sub>H :: "4 word"
+  err\<^sub>H :: bit
 
 alphabet \<alpha>L =
-  reg\<^sub>L :: int
-  err\<^sub>L :: int
+  reg\<^sub>L :: "4 word"
+  err\<^sub>L :: bit
 
 (* ST defines what states are valid *)
+(*
 definition ST
   where "ST = (reg \<ge> 0 \<and> reg \<le> 255 \<and> err \<ge> 0 \<and> err \<le> 1)\<^sub>e"
+*)
 
 (* DBL doubles the number, if it is low enough to double without overflow *)
 definition DBL
   where "DBL = (reg\<^sup>< \<ge> 0 \<and> reg\<^sup>< \<le> 127 \<and> err\<^sup>< = 0)\<^sub>e \<turnstile>\<^sub>r (reg\<^sup>> = reg\<^sup>< * 2 \<and> err\<^sup>> = 0)\<^sub>e"
 
+value "DBL (\<lparr> ok\<^sub>v = True, \<dots> = \<lparr> reg\<^sub>v = -1, err\<^sub>v = 0 \<rparr> \<rparr>, \<lparr> ok\<^sub>v = False, \<dots> = \<lparr> reg\<^sub>v = 0, err\<^sub>v = 0 \<rparr> \<rparr>)"
+
+value "ucast (drop_bit 4 (240::8 word)) :: 4 word"
+value "ucast (take_bit 4 (15::8 word)) :: 4 word"
+
 (* A view of the high nibble *)
 definition Hv
-  where "Hv = OK (((vu:reg\<^sub>H = floor (sys:reg / 16)) \<and> (vu:err\<^sub>H = sys:err))\<^sub>e \<up> \<^bold>v\<^sub>D)"
+  where "Hv = OK (((vu:reg\<^sub>H = (ucast (drop_bit 4 sys:reg))) \<and> (vu:err\<^sub>H = sys:err))\<^sub>e \<up> \<^bold>v\<^sub>D)"
 
 (* A view of the low nibble *)
 definition Lv
-  where "Lv = OK (((vu:reg\<^sub>L = sys:reg mod 16) \<and> (vu:err\<^sub>L = sys:err))\<^sub>e \<up> \<^bold>v\<^sub>D)"
+  where "Lv = OK (((vu:reg\<^sub>L = (ucast (take_bit 4 sys:reg))) \<and> (vu:err\<^sub>L = sys:err))\<^sub>e \<up> \<^bold>v\<^sub>D)"
 
 (*
 Consider an example where the register stores the value 60
@@ -49,7 +61,7 @@ Here is an observation on the final state, with this value
 
 definition \<Phi> where "\<Phi> = (reg = 60 \<and> err = 0)\<^sub>e"
 
-lemma "Hv is VHD"
+lemma hv_is_vhd: "Hv is VHD"
   by (pred_auto_banks add: Hv_def)
 
 lemma "Lv is VHD"
@@ -62,15 +74,45 @@ lemma "Lv is VHD"
       LLLL = 1100(b2) = 12(b10)
 *)
 
-lemma "(((L (Hv \<down> \<^bold>v\<^sub>D) (\<Delta> \<Phi>))) \<down> vu\<^sup>2) = (reg\<^sub>H\<^sup>> = 3 \<and> err\<^sub>H\<^sup>> = 0)\<^sub>e"
+lemma "(((L (Hv \<down> \<^bold>v\<^sub>D) (\<Delta> \<Phi>))) \<down> vu\<^sup>2) = \<Delta> (reg\<^sub>H = 3 \<and> err\<^sub>H = 0)\<^sub>e"
   by (pred_auto_banks add: Hv_def \<Phi>_def)
 
-lemma "(((L (Lv \<down> \<^bold>v\<^sub>D) (\<Delta> \<Phi>))) \<down> vu\<^sup>2) = (reg\<^sub>L\<^sup>> = 12 \<and> err\<^sub>L\<^sup>> = 0)\<^sub>e"
+lemma "(((L (Lv \<down> \<^bold>v\<^sub>D) (\<Delta> \<Phi>))) \<down> vu\<^sup>2) = \<Delta> (reg\<^sub>L = 12 \<and> err\<^sub>L = 0)\<^sub>e"
   by (pred_auto_banks add: Lv_def \<Phi>_def)
 
+term "(as_design_view(
+     ((reg\<^sub>H\<^sup>< \<ge> 0 \<and> reg\<^sub>H\<^sup>< \<le> 7 \<and> err\<^sub>H\<^sup>< = 0)\<^sub>e)
+     \<turnstile>\<^sub>r
+     ((((reg\<^sub>H\<^sup>> = (reg\<^sub>H\<^sup>< * 2)) \<or> (reg\<^sub>H\<^sup>> = ((reg\<^sub>H\<^sup>< * 2) + 1))) \<and> err\<^sub>H\<^sup>> = 0)\<^sub>e)
+  ))"
+
+value "(255::8 word) = (-1::8 word)"
+(*
+lemma "(L\<^sub>D (Hv) (DBL)) (
+        \<lparr> ok\<^sub>v = True, \<dots> = \<lparr> sys\<^sub>v = \<lparr> reg\<^sub>v = 255, err\<^sub>v = 0 \<rparr>, vu\<^sub>v = \<lparr> reg\<^sub>H\<^sub>v = 0, err\<^sub>H\<^sub>v = 0 \<rparr> \<rparr> \<rparr>
+        ,\<lparr> ok\<^sub>v = False, \<dots> = \<lparr> sys\<^sub>v = \<lparr> reg\<^sub>v = 255, err\<^sub>v = 0 \<rparr>, vu\<^sub>v = \<lparr> reg\<^sub>H\<^sub>v = 0, err\<^sub>H\<^sub>v = 0 \<rparr> \<rparr> \<rparr>
+    )"
+  apply (pred_auto_banks add: Hv_def DBL_def)
+  quickcheck
+  apply transfer
+  apply simp
+  *)
+
+term "(L\<^sub>D (Hv) (DBL))"
+
+find_theorems "take_bit ?n (drop_bit ?m ?P)"
+
+
+lemma "L\<^sub>p ((vu:reg\<^sub>H = (ucast (drop_bit 4 sys:reg))) \<and> (vu:err\<^sub>H = sys:err))\<^sub>e (reg \<ge> 0 \<and> reg \<le> 127 \<and> err = 0)\<^sub>e  = (reg\<^sub>H \<ge> 0 \<and> reg\<^sub>H \<le> 7 \<and> err\<^sub>H = 0)\<^sub>e"
+  apply (pred_simp add: banks_defs)
+  apply (simp add: drop_bit_eq_div word_le_nat_alt unat_div_distrib div_le_mono)
+
+
+
 (* TODO is this right? *)
-lemma "
-  (L\<^sub>D (Hv \<and> (ST \<up> sys \<up> \<^bold>v\<^sub>D)) (DBL))
+lemma
+ "
+  (L\<^sub>D (Hv) (DBL))
   =
   (as_design_view(
     ((reg\<^sub>H\<^sup>< \<ge> 0 \<and> reg\<^sub>H\<^sup>< \<le> 7 \<and> err\<^sub>H\<^sup>< = 0)\<^sub>e)
@@ -78,13 +120,55 @@ lemma "
      ((((reg\<^sub>H\<^sup>> = (reg\<^sub>H\<^sup>< * 2)) \<or> (reg\<^sub>H\<^sup>> = ((reg\<^sub>H\<^sup>< * 2) + 1))) \<and> err\<^sub>H\<^sup>> = 0)\<^sub>e)
   ))
   "
-  apply (pred_auto_banks add: Hv_def DBL_def ST_def)
-  sorry
-
-lemma "(L\<^sub>D (Lv \<and> (ST \<up> sys \<up> \<^bold>v\<^sub>D)) (DBL)) = true"
-  apply (pred_auto_banks add: DBL_def Lv_def ST_def)
-  by (metis zero_neq_one)
+  apply (unfold DBL_def)
+  apply (subst view_local_design)
+    apply (fact hv_is_vhd)
+   apply (simp add: Hv_def banks_defs)
+   apply pred_simp
   
+  apply (pred_auto_banks add: Hv_def DBL_def)
+                      apply (transfer, auto)
+  quickcheck
+
+lemma "(L\<^sub>D (Hv) (DBL)) (
+   \<lparr> ok\<^sub>v = True, \<dots> = \<lparr> sys\<^sub>v = \<lparr> reg\<^sub>v = 255, err\<^sub>v = 0 \<rparr>, vu\<^sub>v = \<lparr> reg\<^sub>H\<^sub>v = 0, err\<^sub>H\<^sub>v = 0 \<rparr> \<rparr>  \<rparr>
+  ,\<lparr> ok\<^sub>v = False, \<dots> = \<lparr> sys\<^sub>v = \<lparr> reg\<^sub>v = 255, err\<^sub>v = 0 \<rparr>, vu\<^sub>v = \<lparr> reg\<^sub>H\<^sub>v = 0, err\<^sub>H\<^sub>v = 0 \<rparr> \<rparr>  \<rparr>
+)"
+  apply (pred_auto_banks add: Hv_def DBL_def)
+  apply transfer
+  by (metis not_mod_2_eq_0_eq_1 take_bit_eq_mod take_bit_length_eq word_mod_def word_of_int_eq_iff)
+
+lemma "(reg\<^sub>H \<ge> 0 \<and> reg\<^sub>H \<le> 7 \<and> err\<^sub>H = 0)\<^sub>e \<lparr> reg\<^sub>H\<^sub>v = 0, err\<^sub>H\<^sub>v = 0 \<rparr>"
+
+lemma " (as_design_view(
+    ((reg\<^sub>H\<^sup>< \<ge> 0 \<and> reg\<^sub>H\<^sup>< \<le> 7 \<and> err\<^sub>H\<^sup>< = 0)\<^sub>e)
+     \<turnstile>\<^sub>r
+     ((((reg\<^sub>H\<^sup>> = (reg\<^sub>H\<^sup>< * 2)) \<or> (reg\<^sub>H\<^sup>> = ((reg\<^sub>H\<^sup>< * 2) + 1))) \<and> err\<^sub>H\<^sup>> = 0)\<^sub>e)
+  )) (
+   \<lparr> ok\<^sub>v = True, \<dots> = \<lparr> sys\<^sub>v = \<lparr> reg\<^sub>v = 255, err\<^sub>v = 0 \<rparr>, vu\<^sub>v = \<lparr> reg\<^sub>H\<^sub>v = 0, err\<^sub>H\<^sub>v = 0 \<rparr> \<rparr>  \<rparr>
+  ,\<lparr> ok\<^sub>v = False, \<dots> = \<lparr> sys\<^sub>v = \<lparr> reg\<^sub>v = 255, err\<^sub>v = 0 \<rparr>, vu\<^sub>v = \<lparr> reg\<^sub>H\<^sub>v = 0, err\<^sub>H\<^sub>v = 0 \<rparr> \<rparr>  \<rparr>
+  )"
+  apply (pred_auto_banks add: Hv_def DBL_def)
+
+
+lemma "
+  (L ((Hv \<down> \<^bold>v\<^sub>D)) (DBL \<down> \<^bold>v\<^sub>D\<^sup>2)) \<down> vu\<^sup>2
+  =
+  (
+    ((reg\<^sub>H\<^sup>< \<ge> 0 \<and> reg\<^sub>H\<^sup>< \<le> 7 \<and> err\<^sub>H\<^sup>< = 0)\<^sub>e)
+     \<turnstile>\<^sub>r
+     ((((reg\<^sub>H\<^sup>> = (reg\<^sub>H\<^sup>< * 2)) \<or> (reg\<^sub>H\<^sup>> = ((reg\<^sub>H\<^sup>< * 2) + 1))) \<and> err\<^sub>H\<^sup>> = 0)\<^sub>e)
+  ) \<down> \<^bold>v\<^sub>D\<^sup>2
+  "
+  apply (pred_auto_banks add: Hv_def DBL_def)
+  quickcheck
+
+lemma "(L\<^sub>D (Lv) (DBL)) = true"
+  apply (pred_auto_banks add: DBL_def Lv_def)
+  apply transfer
+  nitpick
+  apply smt
+
 
 (* DBL2 doubles the number, if it is low enough to double without overflow, but unlike DBL, it
 explicitly defines the behaviour in the overflow case. If overflow is detected, then the err bit is
@@ -98,6 +182,8 @@ definition DBL2
 
 (* DBL is refined by DBL2 *)
 lemma "DBL \<sqsubseteq> DBL2"
-  by (pred_auto_banks add: DBL_def DBL2_def)
+  apply (pred_auto_banks add: DBL_def DBL2_def)
+  by (transfer;auto)+
+    
 
 end
